code/style-experiments/Hacl.Impl.Aes.Generic.fst
@@ -16,27 +16,17 @@ noextract inline_for_extraction let nr =  10 // 10, 12, or 14 for 128/192/256
 type skey  = lbytes 16
 type skey256  = lbytes 32
 
-inline_for_extraction
-let ctxlen (m:m_spec) =  nlen m + (15 `op_Multiply` klen m)
-
+unfold
 type keyr (m:m_spec) =  lbuffer (stelem m) (9 `op_Multiply` klen m)
+unfold
 type keyex (m:m_spec) = lbuffer (stelem m) (15 `op_Multiply` klen m) // Saving space for AES-256
-type aes_ctx (m:m_spec) = lbuffer (stelem m) (ctxlen m) 
-
-inline_for_extraction
-let get_nonce (#m:m_spec) (ctx:aes_ctx m) = sub ctx (size 0) (size (nlen m))
-inline_for_extraction
-let get_kex (#m:m_spec) (ctx:aes_ctx m) = sub ctx (size (nlen m)) (size 15 
-*. size (klen m))
-
-inline_for_extraction
-let create_ctx (m:m_spec) = create (elem_zero m) (size (ctxlen m))
 
 inline_for_extraction
 val add_round_key: #m:m_spec -> st:state m -> key:key1 m -> ST unit
 			     (requires (fun h -> live h st /\ live h key))
 			     (ensures (fun h0 _ h1 -> live h1 st /\ live h1 key /\ modifies (loc_buffer st) h0 h1))
-let add_round_key #m st key = xor_state_key1 st key
+let add_round_key #m st key = xor_state_key1 #m st key
+
 
 inline_for_extraction
 val enc_rounds: #m:m_spec -> st:state m -> key:keyr m -> n:size_t -> ST unit
@@ -45,7 +35,7 @@ val enc_rounds: #m:m_spec -> st:state m -> key:keyr m -> n:size_t -> ST unit
 let enc_rounds #m st key n = 
     let h0 = ST.get() in
     loop_nospec #h0 n st 
-      (fun i -> let sub_key = sub key i (size (klen m)) in aes_enc st sub_key)
+      (fun i -> let sub_key = sub key (i *. size (klen m)) (size (klen m)) in aes_enc #m st sub_key)
 
 
 inline_for_extraction
@@ -56,11 +46,11 @@ let block_cipher #m st key n =
     let inner_rounds = n -. size 1 in
     let klen = size (klen m) in
     let k0 = sub key (size 0) klen in
-    let kr = sub key (size 1) (inner_rounds *. klen) in
-    let kn = sub key (size 10) klen in
-    add_round_key st k0;
-    enc_rounds st kr (n -. size 1);
-    aes_enc_last st kn
+    let kr = sub key klen (inner_rounds *. klen) in
+    let kn = sub key (n *. klen) klen in
+    add_round_key #m st k0;
+    enc_rounds #m st kr (n -. size 1);
+    aes_enc_last #m st kn
 
 
 let rcon =  gcreateL [u8(0x8d); u8(0x01); u8(0x02); u8(0x04); u8(0x08); u8(0x10); u8(0x20); u8(0x40); u8(0x80); u8(0x1b); u8(0x36)]
@@ -73,7 +63,8 @@ val key_expansion128: #m:m_spec -> keyx:keyex m -> key:lbytes 16 -> ST unit
 			     (ensures (fun h0 _ h1 -> live h1 keyx /\ live h1 key /\ modifies (loc_buffer keyx) h0 h1))
 [@ CInline ]
 let key_expansion128 #m keyx key = 
-    load_key1 (sub keyx (size 0) (size (klen m))) key;
+    let klen = size (klen m) in
+    load_key1 (sub keyx (size 0) klen) key;
     let h0 = ST.get() in
     (* I WOULD LIKE TO HAVE A LOOP HERE BUT AES_KEYGEN_ASSIST INSISTS ON AN IMMEDIATE RCON *)
     (* MAYBE WE SHOULD UNROLL ONLY THIS LOOP *)
@@ -82,112 +73,114 @@ let key_expansion128 #m keyx key =
        let prev = sub keyx i (size 1) in
        let next = sub keyx (i +. size 1) (size 1) in
        aes_keygen_assist next rcon.(i +. size 1);
-       key_expansion_step next prev)
+       key_expansion_step #m next prev)
 		     *)
-       let prev = sub keyx (size 0) (size 1) in
-       let next = sub keyx (size 1) (size 1) in
-       aes_keygen_assist next prev (u8 0x01);
-       key_expansion_step next prev;
-       let prev = sub keyx (size 1) (size 1) in
-       let next = sub keyx (size 2) (size 1) in
-       aes_keygen_assist next prev (u8 0x02);
-       key_expansion_step next prev;
-       let prev = sub keyx (size 2) (size 1) in
-       let next = sub keyx (size 3) (size 1) in
-       aes_keygen_assist next prev (u8 0x04);
-       key_expansion_step next prev;
-       let prev = sub keyx (size 3) (size 1) in
-       let next = sub keyx (size 4) (size 1) in
-       aes_keygen_assist next prev (u8 0x08);
-       key_expansion_step next prev;
-       let prev = sub keyx (size 4) (size 1) in
-       let next = sub keyx (size 5) (size 1) in
-       aes_keygen_assist next prev (u8 0x10);
-       key_expansion_step next prev;
-       let prev = sub keyx (size 5) (size 1) in
-       let next = sub keyx (size 6) (size 1) in
-       aes_keygen_assist next prev (u8 0x20);
-       key_expansion_step next prev;
-       let prev = sub keyx (size 6) (size 1) in
-       let next = sub keyx (size 7) (size 1) in
-       aes_keygen_assist next prev (u8 0x40);
-       key_expansion_step next prev;
-       let prev = sub keyx (size 7) (size 1) in
-       let next = sub keyx (size 8) (size 1) in
-       aes_keygen_assist next prev (u8 0x80);
-       key_expansion_step next prev;
-       let prev = sub keyx (size 8) (size 1) in
-       let next = sub keyx (size 9) (size 1) in
-       aes_keygen_assist next prev (u8 0x1b);
-       key_expansion_step next prev;
-       let prev = sub keyx (size 9) (size 1) in
-       let next = sub keyx (size 10) (size 1) in
-       aes_keygen_assist next prev (u8 0x36);
-       key_expansion_step next prev
+       let prev = sub keyx (size 0) klen in
+       let next = sub keyx klen klen in
+       aes_keygen_assist #m next prev (u8 0x01);
+       key_expansion_step #m next prev;
+       let prev = sub keyx klen klen in
+       let next = sub keyx (size 2 *. klen) klen in
+       aes_keygen_assist #m next prev (u8 0x02);
+       key_expansion_step #m next prev;
+       let prev = sub keyx (klen *. size 2) (klen) in
+       let next = sub keyx (klen *. size 3) (klen) in
+       aes_keygen_assist #m next prev (u8 0x04);
+       key_expansion_step #m next prev;
+       let prev = sub keyx (klen *. size 3) (klen) in
+       let next = sub keyx (klen *. size 4) (klen) in
+       aes_keygen_assist #m next prev (u8 0x08);
+       key_expansion_step #m next prev;
+       let prev = sub keyx (klen *. size 4) (klen) in
+       let next = sub keyx (klen *. size 5) (klen) in
+       aes_keygen_assist #m next prev (u8 0x10);
+       key_expansion_step #m next prev;
+       let prev = sub keyx (klen *. size 5) (klen) in
+       let next = sub keyx (klen *. size 6) (klen) in
+       aes_keygen_assist #m next prev (u8 0x20);
+       key_expansion_step #m next prev;
+       let prev = sub keyx (klen *. size 6) (klen) in
+       let next = sub keyx (klen *. size 7) (klen) in
+       aes_keygen_assist #m next prev (u8 0x40);
+       key_expansion_step #m next prev;
+       let prev = sub keyx (klen *. size 7) (klen) in
+       let next = sub keyx (klen *. size 8) (klen) in
+       aes_keygen_assist #m next prev (u8 0x80);
+       key_expansion_step #m next prev;
+       let prev = sub keyx (klen *. size 8) (klen) in
+       let next = sub keyx (klen *. size 9) (klen) in
+       aes_keygen_assist #m next prev (u8 0x1b);
+       key_expansion_step #m next prev;
+       let prev = sub keyx (klen *. size 9) (klen) in
+       let next = sub keyx (klen *. size 10) (klen) in
+       aes_keygen_assist #m next prev (u8 0x36);
+       key_expansion_step #m next prev
        
 
+inline_for_extraction
 val key_expansion256: #m:m_spec -> keyx:keyex m -> key:lbytes 32 -> ST unit
 			     (requires (fun h -> live h keyx /\ live h key))
 			     (ensures (fun h0 _ h1 -> live h1 keyx /\ live h1 key /\ modifies (loc_buffer keyx) h0 h1))
 let key_expansion256 #m keyx key = 
-    load_key1 (sub keyx (size 0) (size (klen m))) (sub key (size 0) (size 16));
-    load_key1 (sub keyx (size (klen m)) (size (klen m))) (sub key (size 16) (size 16));
+    let klen = size (klen m) in
+    load_key1 (sub keyx (size 0) klen) (sub key (size 0) (size 16));
+    load_key1 (sub keyx klen klen) (sub key (size 16) (size 16));
     let h0 = ST.get() in
-    (* I WOULD LIKE TO HAVE A LOOP HERE BUT AES_KEYGEN_ASSIST INSISTS ON AN IMMEDIATE RCON *)
+    (* I WOULD LIKE TO HAVE A LOOP HERE BUT AES_KEYGEN_ASSIST #M INSISTS ON AN IMMEDIATE RCON *)
     (* MAYBE WE SHOULD UNROLL ONLY THIS LOOP *)
-       let prev0 = sub keyx (size 0) (size 1) in
-       let prev1 = sub keyx (size 1) (size 1) in
-       let next0 = sub keyx (size 2) (size 1) in
-       let next1 = sub keyx (size 3) (size 1) in
-       aes_keygen_assist next0 prev1 (u8 0x01);
-       key_expansion_step next0 prev0;
-       aes_keygen_assist next1 next0 (u8 0x00);
-       key_expansion_step2 next1 prev1;
+       let prev0 = sub keyx (size 0) (klen) in
+       let prev1 = sub keyx (klen) (klen) in
+       let next0 = sub keyx (klen *. size 2) (klen) in
+       let next1 = sub keyx (klen *. size 3) (klen) in
+       aes_keygen_assist #m next0 prev1 (u8 0x01);
+       key_expansion_step #m next0 prev0;
+       aes_keygen_assist #m next1 next0 (u8 0x00);
+       key_expansion_step2 #m next1 prev1;
        let prev0 = next0 in
        let prev1 = next1 in
-       let next0 = sub keyx (size 4) (size 1) in
-       let next1 = sub keyx (size 5) (size 1) in
-       aes_keygen_assist next0 prev1 (u8 0x02);
-       key_expansion_step next0 prev0;
-       aes_keygen_assist next1 next0 (u8 0x00);
-       key_expansion_step2 next1 prev1;
+       let next0 = sub keyx (klen *. size 4) (klen) in
+       let next1 = sub keyx (klen *. size 5) (klen) in
+       aes_keygen_assist #m next0 prev1 (u8 0x02);
+       key_expansion_step #m next0 prev0;
+       aes_keygen_assist #m next1 next0 (u8 0x00);
+       key_expansion_step2 #m next1 prev1;
        let prev0 = next0 in
        let prev1 = next1 in
-       let next0 = sub keyx (size 6) (size 1) in
-       let next1 = sub keyx (size 7) (size 1) in
-       aes_keygen_assist next0 prev1 (u8 0x04);
-       key_expansion_step next0 prev0;
-       aes_keygen_assist next1 next0 (u8 0x00);
-       key_expansion_step2 next1 prev1;
+       let next0 = sub keyx (klen *. size 6) (klen) in
+       let next1 = sub keyx (klen *. size 7) (klen) in
+       aes_keygen_assist #m next0 prev1 (u8 0x04);
+       key_expansion_step #m next0 prev0;
+       aes_keygen_assist #m next1 next0 (u8 0x00);
+       key_expansion_step2 #m next1 prev1;
        let prev0 = next0 in
        let prev1 = next1 in
-       let next0 = sub keyx (size 8) (size 1) in
-       let next1 = sub keyx (size 9) (size 1) in
-       aes_keygen_assist next0 prev1 (u8 0x08);
-       key_expansion_step next0 prev0;
-       aes_keygen_assist next1 next0 (u8 0x00);
-       key_expansion_step2 next1 prev1;
+       let next0 = sub keyx (klen *. size 8) (klen) in
+       let next1 = sub keyx (klen *. size 9) (klen) in
+       aes_keygen_assist #m next0 prev1 (u8 0x08);
+       key_expansion_step #m next0 prev0;
+       aes_keygen_assist #m next1 next0 (u8 0x00);
+       key_expansion_step2 #m next1 prev1;
        let prev0 = next0 in
        let prev1 = next1 in
-       let next0 = sub keyx (size 10) (size 1) in
-       let next1 = sub keyx (size 11) (size 1) in
-       aes_keygen_assist next0 prev1 (u8 0x10);
-       key_expansion_step next0 prev0;
-       aes_keygen_assist next1 next0 (u8 0x00);
-       key_expansion_step2 next1 prev1;
+       let next0 = sub keyx (klen *. size 10) (klen) in
+       let next1 = sub keyx (klen *. size 11) (klen) in
+       aes_keygen_assist #m next0 prev1 (u8 0x10);
+       key_expansion_step #m next0 prev0;
+       aes_keygen_assist #m next1 next0 (u8 0x00);
+       key_expansion_step2 #m next1 prev1;
        let prev0 = next0 in
        let prev1 = next1 in
-       let next0 = sub keyx (size 12) (size 1) in
-       let next1 = sub keyx (size 13) (size 1) in
-       aes_keygen_assist next0 prev1 (u8 0x20);
-       key_expansion_step next0 prev0;
-       aes_keygen_assist next1 next0 (u8 0x00);
-       key_expansion_step2 next1 prev1;
+       let next0 = sub keyx (klen *. size 12) (klen) in
+       let next1 = sub keyx (klen *. size 13) (klen) in
+       aes_keygen_assist #m next0 prev1 (u8 0x20);
+       key_expansion_step #m next0 prev0;
+       aes_keygen_assist #m next1 next0 (u8 0x00);
+       key_expansion_step2 #m next1 prev1;
        let prev0 = next0 in
        let prev1 = next1 in
-       let next0 = sub keyx (size 14) (size 1) in
-       aes_keygen_assist next0 prev1 (u8 0x40);
-       key_expansion_step next0 prev0
+       let next0 = sub keyx (klen *. size 14) (klen) in
+       aes_keygen_assist #m next0 prev1 (u8 0x40);
+       key_expansion_step #m next0 prev0
     
 
 inline_for_extraction
@@ -197,7 +190,7 @@ val aes128_init: #m:m_spec -> ctx:aes_ctx m -> key:skey -> nonce:lbytes 12 -> ST
 let aes128_init #m ctx key nonce = 
   let kex = get_kex ctx in
   let n = get_nonce ctx in
-  key_expansion128 kex key ; 
+  key_expansion128 #m kex key ; 
   load_nonce #m n nonce
 
 inline_for_extraction
@@ -207,7 +200,7 @@ val aes256_init: #m:m_spec -> ctx:aes_ctx m -> key:skey -> nonce:lbytes 12 -> ST
 let aes256_init #m ctx key nonce = 
   let kex = get_kex ctx in
   let n = get_nonce ctx in
-  key_expansion256 kex key ; 
+  key_expansion256 #m kex key ; 
   load_nonce #m n nonce
 
 
@@ -220,9 +213,9 @@ let aes128_key_block #m kb ctx counter =
     let kex = get_kex ctx in
     let n = get_nonce ctx in
     let st = create_state #m in
-    load_state st n counter;
-    block_cipher st kex (size 10);
-    store_block0 kb st;
+    load_state #m st n counter;
+    block_cipher #m st kex (size 10);
+    store_block0 #m kb st;
     pop_frame()
     
 
@@ -234,11 +227,11 @@ val aes_update4: #m:m_spec -> out:lbytes 64 -> inp:lbytes 64 -> ctx:aes_ctx m ->
 let aes_update4 #m out inp ctx ctr rounds =
   push_frame();
   let st = create_state #m in
-  let kex = get_kex ctx in
-  let n = get_nonce ctx in
-  load_state st n ctr;
-  block_cipher st kex rounds;
-  xor_block out st inp;
+  let kex = get_kex #m ctx in
+  let n = get_nonce #m ctx in
+  load_state #m st n ctr;
+  block_cipher #m st kex rounds;
+  xor_block #m out st inp;
   pop_frame()
 
 inline_for_extraction
@@ -254,7 +247,7 @@ let aes_ctr #m out inp len ctx counter rounds =
       let ctr = counter +. (i *. size 4) in
       let ib = sub inp (i *. size 64) (size 64) in
       let ob = sub out (i *. size 64) (size 64) in
-      aes_update4 ob ib ctx ctr rounds);
+      aes_update4 #m ob ib ctx ctr rounds);
   let rem = len %. size 64 in
   if (rem >. size 0) then (
       let ctr = counter +. (blocks64 *. size 4) in
@@ -262,7 +255,7 @@ let aes_ctr #m out inp len ctx counter rounds =
       let ob = sub out (blocks64 *. size 64) rem in
       let last = alloca 0uy 64ul in
       blit ib (size 0) last (size 0) rem;
-      aes_update4 last last ctx ctr rounds;
+      aes_update4 #m last last ctx ctr rounds;
       blit last (size 0) ob (size 0) rem);
   pop_frame()
 
@@ -270,8 +263,8 @@ inline_for_extraction
 let aes128_ctr_encrypt (#m:m_spec) out inp in_len k n c = 
   push_frame();
   let ctx = create_ctx m in
-  aes128_init ctx k n;
-  aes_ctr out inp in_len ctx c (size 10);
+  aes128_init #m ctx k n;
+  aes_ctr #m out inp in_len ctx c (size 10);
   pop_frame()
 
 inline_for_extraction
@@ -282,10 +275,10 @@ inline_for_extraction
 let aes256_ctr_encrypt (#m:m_spec) out inp in_len k n c = 
   push_frame();
   let ctx = create_ctx m in
-  aes256_init ctx k n;
-  aes_ctr out inp in_len ctx c (size 14);
+  aes256_init #m ctx k n;
+  aes_ctr #m out inp in_len ctx c (size 14);
   pop_frame()
 
 inline_for_extraction
 let aes256_ctr_decrypt (#m:m_spec) out inp in_len k n c = 
-  aes128_ctr_encrypt #m out inp in_len k n c
+  aes256_ctr_encrypt #m out inp in_len k n c
